* Added a simple guide for executing the ARM instruction set model.
* Interrupts are now masked at the ISA level.
    Previously it was assumed that FIQ and IRQ interrupts were only input when
    the "F" and "I" masks were clear, but this was not enforced by the model.
    The backward compatibility with 26-bit address space has been dropped for
    the "test and compare" instructions.  For example, TSTP pc, rX cannot
    be used to update the CPSR.

examples/arm6/armLib.sml
@@ -67,7 +67,7 @@ fun arm_rws () =
       NUMERAL_ONLY_RULE `n` CONDITION_PASSED_def,CONDITION_PASSED2_def,
       IS_Dabort_def,IS_Reset_def,PROJ_Dabort_def,PROJ_Reset_def,interrupt2exception_def,
       THE_DEF,IS_SOME_DEF,IS_NONE_EQ_NONE,NOT_IS_SOME_EQ_NONE,option_case_ID,option_case_SOME_ID,
-      option_case_def,SOME_11,NOT_SOME_NONE,PROJ_TRIPLE_def,interrupt2exception_def,
+      option_case_def,SOME_11,NOT_SOME_NONE,PROJ_IF_FLAGS_def,interrupt2exception_def,
       NEXT_ARM_def,OUT_ARM_def
       ] rws
 in
